% Thank you Josh Davis for this template!
% https://github.com/jdavis/latex-homework-template/blob/master/homework.tex

\documentclass{article}

\input{ShortcutsAnalysis}

\newcommand{\hmwkTitle}{Lecture\ \#1}

\begin{document}
\bsc{Theorem 3.2.8 - pg 118}

Let x, y $\in$ $\mathbb{R}$

\balist
\item If x $\leq$ y + $\ep$ $\fa$ $\ep$ $>$ $0$, then x $\leq$ y
\item If $|x - y|$ $\leq$ $\ep$ $\fa$ $\ep$ $>$ $0$, then $|x - y|$ $=$ $0$ or, evidently, $x = y$
\elist

\ssc{a)}
If x $\leq$ y + $\ep$ $\fa$ $\ep$ $>$ $0$, then x $\leq$ y
\bgpf

Suppose that:
$$ x > y $$
$$ x - y > 0 $$

\bigskip

Let $$ \ep = \frac{x + y}{2} > 0$$

See that
\[
            \bgsp
                y + \ep  & 
                \\
                &= y + \frac{x + y}{2}
                \\
                &= y + \frac{x}{2} - \frac{y}{2}
                \\
                &= \frac{x}{2} + \frac{y}{2}
                \\
                &< \frac{x}{2} + \frac{x}{2}
                \\
                &< x
                \\
                y + \ep  &< x \prs{1}
            \end{split}
\]

Thus, by contrapositive, the result is true.

\epf
\pagebreak
\ssc{b)}

If $|x - y|$ $\leq$ $\ep$ $\fa$ $\ep$ $>$ $0$, then $|x - y|$ $=$ $0$ or, evidently, $x = y$

\bgpf

Suppose that:

$$|x - y| > 0$$

Let

$$ \ep = \frac{|x - y|}{2} $$

See that

\[
            \bgsp
                &1 > \frac{1}{2}
                \\
                &|x - y| > \frac{1}{2}|x - y|
                \\
                &|x - y| > \epsilon
            \end{split}
\]

Thus, by contrapositive, the result is true.

\epf

\pagebreak

\bsc{Definition 3.2.9}

If x $\in \br$,

\bgeq
  |x|=\begin{cases}
    x, & \text{if $x \geq 0$}.\\
    -x, & \text{if $x < 0$}.
  \end{cases}
\eeq

\bsc{Theorem 3.2.10}
Let x, y $\in \br$ and a $\geq 0$ \\
\\
Then
\balist
\item $|x| \geq 0$
\item $|x| \leq a iff -a \leq x \leq a$
\item $|xy| = |x||y|$
\item $|x + y| \leq |x| + |y|$
\elist

\ssc{a)}
$|x| \geq 0$
\bgpf

Case:
\bilist
\item $x \geq 0$: \\
	then $|x| = x \geq 0$
\item $x < 0 \rar -x > 0$ \\
	then $|x| = -x \geq 0$
\elist

Hence, result
\epf

\ssc{b)}

$|x| \leq a$ iff $-a \leq x \leq a$ \\

Since it's a biconditional, first we prove p $\rar$ q, then q $\rar$ p.
\bgpf

Notice that:
$$ -a \leq -|x|$$
Case:
\bilist
\item $x \geq 0$ \\
	then $0 \leq x = |x|$ \\
	and  $\therefore |x| \leq a$
	
	Also, since $x = |x| \geq 0$,
	$-a \leq x$ or $-a \leq 0$
	$-a \leq x \leq a$
\item $x < 0$
	$|x| = -x \leq a
	x \geq -a
	\therefore -a \leq x
	-a \leq x \leq a$
\elist

Hence, result.

$\lla$

Conversely, we shall prove that q $\rar$ p

\supp{$-a \leq x \leq a$}

Then:

\bilist
\item x $\geq 0$, then $|x| = x \leq a$
\item x $< 0$, then $|x| = -x \leq a$
\elist

Hence, result.

\ssc{c)} $|xy| = |x||y|$

Notice that if x $=$ 0 (p) or y $=$ 0 (q), then $|xy| = 0 = |x||y|$.

WLOG, assume that not [p or q] $=$ not p $\cap$ not q.

\bilist
\item $x > 0$ and $y > 0$
	then $|x| = x$, $|y| = y$
	Also, $xy > 0$
	So, $|xy| = xy = |x||y|$
\item $x < 0$, $y < 0$
	then $|x| = -x, |y| = -y, xy > 0$
	So, $|xy| = xy = -|x|(-|y|) = |x||y|$
\item $x > 0$, $y < 0$ OR $y > 0$, $x < 0$
	WLOG, let $x > 0$, $y < 0$
	$|xy| = |x||y|$
	$|yx| = |y||x|$
	$|x| = x$, $|y| = -y$, $xy < 0$
	So, $|xy| = -(xy)$ \
		$-[|x|(-|y|)]$ \ 
		$-[-|x||y|]$ \
		$|x||y|$ \ 
\elist
	
\ssc{d)} $|x + y| \leq |x| + |y|$ \

\lt{Z $= x + y$, and a $= |x| + |y|$}

If $a \geq 0$, then $|Z| \leq a$ iff $-a \leq Z \leq a$

$-(|x| + |y|) \leq x + y \leq |x| + |y|$ \

From b), since $|x| + |y| \geq 0$, \

\

\wts{$-(|x| + |y|) \leq x + y \leq |x| + |y|$}

Notice: $-|x| \leq x \leq |x|$

$|x| = x$ or $|x| = -x$ or $-|x| = x$ \

\

Then \

$-|x| - |y| \leq x + y \leq |x| + |y|$ \

$-(|x| + |y|) \leq x + y \leq |x| + |y|$

By b), this is equivalent to \

$|x + y| \leq |x| + |y|$

\epf
\end{document}